\documentclass{article}

\usepackage{amsmath,amssymb,amsthm}
\usepackage[margin=0.5in]{geometry}

\setlength{\parindent}{0pt}
\setlength{\parskip}{1.5pt}

\newtheorem{theorem}{Theorem}
\newtheorem{lemma}{Lemma}

\begin{document}

\section{Chapter 1: Basic Properties of Numbers}

\paragraph{Numbers.} Of the first twelve properties in this chapter, the first nine are concerned with the fundamental operations of addition and multiplication.

\begin{tabular}{l l p{4in}}
  (P1) & (Associative law for addition) & $a + (b + c) = (a + b) + c$. \label{p1} \\
  (P2) & (Existence of an additive identity) & $a + 0 = 0 + a = a$. \label{p2} \\
  (P3) & (Existence of additive inverses) & $a + (-a) = (-a) + a = 0$. \label{p3} \\
  (P4) & (Commutative law for addition) & $a + b = b + a$. \label{p4} \\
  (P5) & (Associative law for multiplication) & $a \cdot (b \cdot c) = (a \cdot b) \cdot c$. \label{p5} \\
  (P6) & (Existence of a multiplicative identity) & $a \cdot 1 = 1 \cdot a = a; 1 \neq 0$. \label{p6} \\
  (P7) & (Existence of a multiplicative inverse) & $a \cdot a^{-1} = a^{-1} \cdot a = 1, \text{ for } a \neq 0$. \label{p7} \\
  (P8) & (Commutative law for multiplication) & $a \cdot b = b \cdot a$. \label{p8} \\
  (P9) & (Distributive law) & $a \cdot (b + c) = a \cdot b + a \cdot c$. \label{p9}
\end{tabular}

The last three are concerned with inequalities. Considering the collection of all positive numbers, $P$,

\begin{tabular}{l l p{4in}}
  (P10) & (Trichotomy law) & For every number $a$, one and only one of the following holds: \begin{enumerate}
      \itemsep0em
      \item $a = 0$,
      \item $a$ is in the collection $P$,
      \item $-a$ is in the collection $P$. \label{p10}
    \end{enumerate} \\
  (P11) & (Closure under addition) & If $a$ and $b$ are in $P$, then $a + b$ is in $P$. \\
  (P12) & (Closure under multiplication) & If $a$ and $b$ are in $P$, then $a \cdot b$ is in $P$.
\end{tabular}

\section{Exercises}

\setcounter{subsection}{7}
\subsection{Defining $P$ in terms of $<$}

\paragraph{Problem.} Suppose that P10-12 are replaced by the following properties:

\begin{tabular}{l p{4in}}
  (P'10) & For every number $a$ and $b$, one and only one of the following holds: \begin{enumerate}
      \itemsep0em
      \item $a = b$,
      \item $a < b$,
      \item $b < a$. \label{p'10}
    \end{enumerate} \\
  (P'11) & For any numbers $a$, $b$, and $c$, if $a < b$ and $b < c$, then $a < c$. \label{p'11} \\
  (P'12) & For any numbers $a$, $b$, and $c$, if $a < b$, then $a + c < b + c$. \label{p'12} \\
  (P'13) & For any numbers $a$, $b$, and $c$, if $a < b$ and $0 < c$, then $ac < bc$. \label{p'13} \\
\end{tabular}

Show that P10-12 can then be deduced as theorems.

\paragraph{Solution.} P10 can be deduced by considering P'10 with $b = 0$. Then, for every number $a$, one and only one of the following holds: \begin{enumerate}
    \itemsep0em
    \item $a = 0$,
    \item $a < 0$ i.e. $-a$ is in $P$,
    \item $0 < a$ i.e. $a$ is in $P$.
\end{enumerate}

P11 can be deduced by considering P'12 with $a = 0$. Then, for any numbers $b$ and $c$, if $0 < b$, $0 + c < b + c$. If $0 < c$ too, then $0 < 0 + c < b + c$. Therefore, if $0 < b$ and $0 < c$, $0 < b + c$ i.e. if $b$ and $c$ are in $P$, then $b + c$ is in $P$.

P12 can be deduced by considering P'11 and P'13. From P'11, for any numbers $a$ and $b$, if $0 < a$ and $a < b$, then $0 < b$. Hence, from P'13, for any numbers $a$ and $b$, if $0 < a$ and $0 < b$, then $0 \cdot a < a \cdot b$ i.e. if $a$ and $b$ are in $P$, then $ab$ is in $P$.

\setcounter{subsection}{14}
\subsection{Proving inequalities}

\paragraph{Problem.} Prove that if $x$ and $y$ are not both 0, then \begin{gather*}
  x^2 + xy + y^2 > 0, \\
  x^4 + x^3y + x^2y^2 + xy^3 + y^4 > 0
\end{gather*}.

\paragraph{Solution.} From Problem 1, $x^n - y^n = (x - y)(x^{n-1} + x^{n-2}y + \cdots + xy^{n-2} + y^{n-1})$. Without loss of generality, assume $x > y$. Considering these two inequalities, \begin{gather*}
  x^3 - y^3 > 0, \\
  x^4 - y^4 > 0
\end{gather*} and factorising out $x - y > 0$, \begin{gather*}
  (x - y)(x^2 + xy + y^2) > 0 \iff x^2 + xy + y^2 > 0 \\
  (x - y)(x^3 + x^2y + xy^2 + y^3) > 0 \iff x^3 + x^2y + xy^2 + y^3 > 0.
\end{gather*} This concludes the proof.

\setcounter{subsection}{15}
\subsection{Proving properties of $(x + y )^n$}

\paragraph{Problem (a).} Show that \begin{gather*}
  (x + y)^2 = x^2 + y^2 \text{ only when } x = 0 \text{ or } y = 0, \\
  (x + y)^3 = x^3 + y^3 \text{ only when } x = 0 \text{ or } y = 0 \text{ or } x = -y.
\end{gather*}

\paragraph{Solution (a).} $(x + y)^2 = x^2 + 2xy + y^2$. Clearly, for $(x + y)^2 = x^2 + y^2$, $2xy = 0$ which implies $x = 0$ or $y = 0$. Similarly, $(x + y)^3 = x^3 + 3x^2y + 3xy^2 + y^3$, and for $(x + y)^3 = x^3 + y^3$, $3x^2y + 3xy^2 = 3xy(x + y) = 0$ which implies $x = 0$ or $y = 0$ or $x = -y$.

\paragraph{Problem (b).} Using the fact that \begin{equation*}
  x^2 + 2xy + y^2 = (x + y)^2 \geq 0,
\end{equation*} show that $4x^2 + 6xy + 4y^2 > 0$ unless $x$ and $y$ are both 0.

\paragraph{Solution (b).} $4x^2 + 6xy + 4y^2 = (x^2 + y^2) + 3(x + y)^2 \geq x^2 + y^2 + 0 = x^2 + y^2$. However, $x^2 + y^2 = 0$ only when $x$ and $y$ are both 0; otherwise, $x^2 + y^2 > 0$.  Hence, it is clear that $4x^2 + 6xy + 4y^2 > 0$ unless $x$ and $y$ are both 0.

\paragraph{Problem (c).} Use part (b) to find out when $(x + y)^4 = x^4 + y^4$.

\paragraph{Solution (c).} $(x + y)^4 = x^4 + 4x^3y + 6x^2y^2 + 4xy^3 + y^4 = (x^4 + y^4) + xy(4x^2 + 6xy + 4y^2)$. It is now obvious that for $(x + y)^4 = x^4 + y^4$, $xy(4x^2 + 6xy + 4y^2) = 0$ which implies $x = 0$ or $y = 0$ or $4x^2 + 6xy + 4y^2 = 0$. From (b), $4x^2 + 6xy + 4y^2 > 0$ unless $x$ and $y$ are both 0. Hence, $(x + y)^4 = x^4 + y^4$ only when $x = 0$ or $y = 0$.

\paragraph{Problem (d).} Find out when $(x + y)^5 = x^5 + y^5$.

\paragraph{Solution (d).} $(x + y)^5 = x^5 + 5x^4y + 10x^3y^2 + 10x^2y^3 + 5xy^4 + y^5 = (x^5 + y^5) + 5xy(x^3 + 2x^2y + 2xy^2 + y^3)$. It is clear that for $(x + y)^5 = x^5 + y^5$, $5xy(x^3 + 2x^2y + 2xy^2 + y^3) = 0$ which implies $x = 0$, $y = 0$ or $x^3 + 2x^2y + 2xy^2 + y^3 = 0$. The problem simplifies to solving $x^3 + 2x^2y + 3xy^2 + y^3 = 0$ if $xy \neq 0$.

Considering $(x + y)^3 = x^3 + 3x^2y + 3xy^2 + y^3 = (x^3 + 2x^2y + 2xy^2 + y^3) + xy(x + y)$, for $x^3 + 2x^2y + 2xy^2 + y^3 = 0$ if $xy \neq 0$, $(x + y)^3 = xy(x + y)$. Since $xy \neq 0$, $x = -y$.

Hence, $(x + y)^5 = x^5 + y^5$ only when $x = 0$ or $y = 0$ or $x = -y$.

\setcounter{subsection}{20}
\subsection{Proving inequalities with modulus}

\paragraph{Problem.} Prove that if \begin{equation*}
  |x - x_0| < min\left(\frac{\epsilon}{2(|y_0| + 1)}, 1\right) \text{ and } |y - y_0| < \frac{\epsilon}{2(|x_0| + 1)},
\end{equation*} then $|xy - x_0y_0| < \epsilon$.

\paragraph{Solution.} The problem can be rewritten in terms of three inequalities \begin{align*}
  |x - x_0| &< \frac{\epsilon}{2(|y_0| + 1)}, \\
  |x - x_0| &< 1, \\
  |y - y_0| &< \frac{\epsilon}{2(|x_0| + 1)}
\end{align*} with the first and third inequality further rewritten into \begin{align*}
  (|x_0| + 1)|y - y_0| &< \frac{\epsilon}{2}, \\
  (|y_0| + 1)|x - x_0| &< \frac{\epsilon}{2}.
\end{align*}

By the reverse triangle inequality, $|x| - |x_0| \leq |x - x_0| < 1$ which yields $|x| < |x_0| + 1$. Rewritting $xy - x_0y_0 = x(y - y_0) + y_0(x - x_0)$ and applying the triangle inequality, \begin{align*}
  |xy - x_0y_0| &\leq |x(y - y_0)| + |y_0(x - x_0)| \\
                &= |x||y - y_0| + |y_0||x - x_0| \\
                &< (|x_0| + 1)|y - y_0| + |y_0||x - x_0| \\
                &< (|x_0| + 1)|y - y_0| + (|y_0| + 1)|x - x_0| \\
                &< \frac{\epsilon}{2} + \frac{\epsilon}{2} \\
                &= \epsilon.
\end{align*}

\setcounter{subsection}{21}
\subsection{Proving inequalities with modulus and reciprocals}

\paragraph{Problem.} Prove that if $y_0 \neq 0$ and \begin{equation*}
  |y - y_0| < min\left(\frac{|y_0|}{2}, \frac{\epsilon|y_0|^2}{2}\right),
\end{equation*} then $y \neq 0$ and \begin{equation*}
  \left|\frac{1}{y} - \frac{1}{y_0}\right| < \epsilon.
\end{equation*}

\paragraph{Solution.} From the assumption, since $|y - y_0| < \frac{\epsilon|y_0|^2}{2}$, \begin{align*}
  \left|\frac{1}{y} - \frac{1}{y_0}\right| &= \frac{|y_0 - y|}{|yy_0|} \\
                                           &= \frac{|y - y_0|}{|y||y_0|} \\
                                           &< \frac{\frac{\epsilon|y_0|^2}{2}}{|y||y_0|} \\
                                           &= \frac{\epsilon|y_0|}{2|y|}
\end{align*}

By the triangle inequality, $|y_0| = |(y_0 - y) + y| \leq |y_0 - y| + |y| = |y - y_0| + |y|$. Then, $|y| = |y_0| - |y - y_0|$. From the assumption, $|y - y_0| < \frac{|y_0|}{2}$ which leads to $|y| > |y_0| - \frac{|y_0|}{2} = \frac{|y_0|}{2} \iff 2|y| > |y_0|$. Hence, $\frac{\epsilon|y_0|}{2|y|} < \frac{\epsilon|y_0|}{|y_0|} = \epsilon$.

\setcounter{subsection}{22}
\subsection{Combining Q21 and Q22}

\paragraph{Problem.} Replace the question marks in the following statement by expressions involving $\epsilon$, $x_0$, and $y_0$ so that the conclusion will be true:

If $y_0 \neq 0$ and \begin{equation*}
  |y - y_0| < ? \text{ and } |x - x_0| < ?
\end{equation*} then $y \neq 0$ and \begin{equation*}
  \left|\frac{x}{y} - \frac{x_0}{y_0}\right| < \epsilon.
\end{equation*}

\paragraph{Solution.} Replacing $y$ and $y_0$ with $\frac{1}{y}$ and $\frac{1}{y_0}$ respectively in the result proven by Q21, if \begin{equation*}
  |x - x_0| < min\left(\frac{\epsilon}{2(|\frac{1}{y_0}| + 1)}, 1\right) \text{ and } \left|\frac{1}{y} - \frac{1}{y_0}\right| < \frac{\epsilon}{2(|x_0| + 1)}
\end{equation*} then $|x(\frac{1}{y}) - x_0(\frac{1}{y_0})| = \left|\frac{x}{y} - \frac{x_0}{y_0}\right| < \epsilon$ which is what we are looking to prove.

To express the second inequality in terms of $|y - y_0|$, $\epsilon$ must be substituted with $\frac{\epsilon}{2(|x_0| + 1)}$ in the result proven by Q22 which leads to \begin{equation*}
  |y - y_0| < min\left(\frac{|y_0|}{2}, \frac{\epsilon|y_0|^2}{4(|x_0| + 1)}\right).
\end{equation*} Therefore, this proves that if $y_0 \neq 0$ and \begin{equation*}
  |x - x_0| < min\left(\frac{\epsilon}{2(|\frac{1}{y_0}| + 1)}, 1\right) \text{ and } |y - y_0| < min\left(\frac{|y_0|}{2}, \frac{\epsilon|y_0|^2}{4(|x_0| + 1)}\right)
\end{equation*} then $y \neq 0$ and \begin{equation*}
  \left|\frac{x}{y} - \frac{x_0}{y_0}\right| < \epsilon.
\end{equation*}

\setcounter{subsection}{23}
\subsection{Placement of parentheses in a sum}

\paragraph{Problem.} Let us agree, for definiteness, that $a_1 + \cdots + a_n$ will denote \begin{equation*}
  a_1 + (a_2 + (a_3 + \cdots + (a_{n-2} + (a_{n-1} + a_n)))\cdots).
\end{equation*} Thus $a_1 + a_2 + a_3$ denotes $a_1 + (a_2 + a_3)$, and $a_1 + a_2 + a_3 + a_4$ denotes $a_1 + (a_2 + (a_3 + a_4))$, etc.

\paragraph{Problem (a).} Prove that \begin{equation*}
  (a_1 + \cdots + a_k) + a_{k+1} = a_1 + \cdots + a_{k+1}.
\end{equation*}

\paragraph{Solution (a).} The base case $k = 1$ is trivial, since $(a_1) + a_2 = a_1 + a_2$.

Assuming that $(a_1 + \cdots + a_{k-1}) + a_k = a_1 + \cdots + a_k$ for some $k \geq 2$, \begin{align*}
  (a_1 + \cdots + a_k) + a_{k+1} &= ((a_1 + \cdots + a_{k-1}) + a_k) + a_{k+1} \text{ (by assumption)} \\
                                 &= (a_1 + \cdots + a_{k-1}) + (a_k + a_{k+1}) \text{ (by P1)} \\
                                 &= a_1 + \cdots + a_{k-1} + (a_k + a_{k+1}) \text{ (by assumption)} \\
                                 &= a_1 + \cdots + a_{k+1} \text{ (by the definition of } a_1 + \cdots + a_{k+1} \text{)}
\end{align*} This proves the inductive hypothesis.

\paragraph{Problem (b).} Prove that if $n \geq k$, then \begin{equation*}
  (a_1 + \cdots + a_k) + (a_{k+1} + \cdots + a_n) = a_1 + \cdots + a_n.
\end{equation*}

\paragraph{Solution (b).} The base case $n = k$ is trivial.

Assuming that $(a_1 + \cdots + a_k) + (a_{k+1} + \cdots + a_n) = a_1 + \cdots + a_n$ for some $n \geq k + 1$, \begin{align*}
  (a_1 + \cdots + a_k) + (a_{k+1} + \cdots + a_n + a_{n+1}) &= (a_1 + \cdots + a_k) + ((a_{k+1} + \cdots + a_n) + a_{n+1}) \text{ (from (a))} \\
                                                            &= ((a_1 + \cdots + a_k) + (a_{k+1} + \cdots + a_n)) + a_{n+1} \text{ (from P1)} \\
                                                            &= (a_1 + \cdots + a_n) + a_{n+1} \text{ (by assumption)} \\
                                                            &= a_1 + \cdots + a_{n+1} \text{ (from (a))}.
\end{align*} This proves the inductive hypothesis.

\paragraph{Problem (c).} Let $s(a_1, \ldots, a_k)$ be some sum formed from $a_1, \ldots, a_k$. Show that \begin{equation*}
  s(a_1, \ldots, a_k) = a_1 + \ldots + a_k.
\end{equation*}

\paragraph{Solution (c).} The base case $k = 1$ is trivial.

Suppose that this statement holds for all sums comprising less than $k$ terms. Then, there must be two sums $s'(a_1, \ldots, a_l)$ and $s''(a_{l+1}, \ldots, a_k)$ with $l < k$ such that \begin{align*}
  s(a_1, \ldots, a_k) &= s'(a_1, \ldots, a_l) + s''(a_{l+1}, \ldots, a_k) \\
                      &= (a_1 + \ldots + a_l) + (a_{l+1} + \ldots + a_k) \text{ (by assumption)} \\
                      &= a_1 + \ldots + a_k \text{ (from (b))}.
\end{align*} This proves the inductive hypothesis.

\end{document}
