\documentclass{article}

\usepackage{amsmath,amssymb,amsthm}
\usepackage[margin=0.5in]{geometry}

\setlength{\parindent}{0pt}
\setlength{\parskip}{1.5pt}

\newtheorem{theorem}{Theorem}
\newtheorem{lemma}{Lemma}

\begin{document}

\section{Chapter 3: Functions}

\paragraph{Functions.} A \textbf{function} is a collection of pairs of numbers with the following properties: if $(a, b)$ and $(a, c)$ are both in the collection, then $b = c$; in other words, the collection must not contain two different pairs with the same first element.

\paragraph{Domain.} If $f$ is a function, the \textbf{domain} of $f$ is the set of all $a$ for which there is some $b$ such that $(a, b)$ is in $f$. If $a$ is in the domain of $f$, it follows from the definition of a function that there is, in fact, a \emph{unique} number $b$ such that $(a, b)$ is in $f$. This unique $b$ is denoted by $f(a)$.

\section{Exercises}

\setcounter{subsection}{9}
\subsection{Finding functions that meet conditions}

\paragraph{Problem (c).} For which functions $b$ and $c$ can we find a function $x$ such that \begin{equation*}
  (x(t))^2 + b(t)x(t) + c(t) = 0
\end{equation*} for all numbers $t$?

\paragraph{Solution (c).} (The scope is limited to real functions.) Applying the quadratic formula, \begin{equation*}
  x(t) = \frac{-b(t) \pm \sqrt{(b(t))^2 - 4(1)(c(t))}}{2(1)}
\end{equation*}. It is clear that for $x(t)$ to be real for all $t$, $(b(t))^2 - 4(1)(c(t)) \geq 0 \iff (b(t))^2 \geq 4c(t)$ for all $t$.

\paragraph{Problem (d).} What conditions must the functions $a$ and $b$ satisfy if there is to be a function $x$ such that \begin{equation*}
  a(t)x(t) + b(t) = 0
\end{equation*} for all numbers $t$? How many such functions $x$ will there be?

\paragraph{Solution (d).} If $x(t) = 0$ for all $t$, then the only condition is $b(t) = 0$ for all $t$. Otherwise, $x = b/a$ and the condition is $a(t) \neq 0$ for all $t$. There will only be one function $x$ in either case.

\setcounter{subsection}{10}
\subsection{Functions that cycle}

\paragraph{Problem (d) (abridged).} Find a function $H$ such that $H(H(x)) = H(x)$ for all numbers $x$, and such that $H(1) = 36, H(2) = \pi/3, H(13) = 47, H(36) = 36, H(\pi/3) = \pi/3, H(47) = 47$.

\paragraph{Solution (d).} It is clear that the six conditions can be expressed as $H(H(1)) = H(1) = 36$, $H(H(2)) = H(2) = \pi/3$ and $H(H(13)) = H(13) = 47$. What is left is to construct a rule for the remaining numbers in the domain. A simple way of constructing a rule that fits the condition $H(H(x)) = H(x)$ would be to yield the number $47 = H(13)$. Hence, the function $H$ can be defined in this manner: \begin{equation*}
  H(x) = \begin{cases}
    36, \text{ if } x = 1 \text{ or } 36 \\
    \pi/3, \text{ if } x = 2 \text{ or } \pi/3 \\
    47, \text{ otherwise.} \\
  \end{cases}
\end{equation*}

\paragraph{Problem (e).} Find a function $H$ such that $H(H(x)) = H(x)$ for all $x$, and such that $H(1) = 7$, $H(17) = 18$.

\paragraph{Solution (e).} Using a similar method to the previous part, one simply needs to impose the condition $H(H(1)) = H(1) = 7$ and to yield the number $18 = H(17)$. The function $H$ can be defined in this manner: \begin{equation*}
  H(x) = \begin{cases}
    7, \text{ if } x = 1 \text{ or } 7 \\
    18, \text{ otherwise} \\
  \end{cases}
\end{equation*}

\setcounter{subsection}{12}
\subsection{Even and odd functions}

\paragraph{Problem (a).} Prove that any function $f$ with domain $\mathbb{R}$ can be written $f = E + O$, where $E$ is even and $O$ is odd. (A function $g$ is \emph{even} if $g(x) = g(-x)$ and \emph{odd} if $g(x) = -g(-x)$.

\paragraph{Solution (a).} Consider $f(x)$ and $f(-x)$: \begin{align*}
  f(x)  &= E(x) + O(x), \\
  f(-x) &= E(-x) + O(-x) \\
        &= E(x) - O(x).
\end{align*} It is clear that $E(x)$ and $O(x)$ can be solved to obtain these two unique solutions: \begin{align*}
  E(x) = \frac{f(x) + f(-x)}{2}, O(x) = \frac{f(x) - f(-x)}{2}.
\end{align*}

\paragraph{Problem (b) (abridged).} Prove that this way of writing $f$ is unique.

\paragraph{Solution (b).} Solved in (a).

\setcounter{subsection}{15}
\subsection{Functions of sums}

Suppose $f$ satisfies $f(x + y) = f(x) + f(y)$ for all $x$ and $y$.

\paragraph{Problem (a).} Prove that $f(x_1 + \cdots + x_n) = f(x_1) + \cdots + f(x_n)$.

\paragraph{Solution (a).} By definition, the base case $n = 2$ is trivially proved. Suppose that the statement holds for $n = k$ for some integer $k \geq 2$. Then, \begin{align*}
  f(x_1 + \cdots + x_k + x_{k+1}) &= f(x_1 + \cdots + x_k) + f(x_{k+1}) \text{ (by definition)} \\
                                  &= (f(x_1) + \cdots + f(x_k)) + f(x_{k+1}) \text{ (by assumption)} \\
                                  &= f(x_1) + \cdots + f(x_{k+1}).
\end{align*} This proves the statement for all $n \geq 2$.

\paragraph{Problem (b) (abridged).} Prove that there is some number $c$ such that $f(x) = cx$ for all rational numbers $x$.

\paragraph{Solution (b).} Let $c = f(1)$. Then, it is clear that $f(n) = cn$ for any natural number $n$.

Since $f(x) + f(0) = f(x + 0) = f(x)$, it follows that $f(0) = 0$. Since $f(x) + f(-x) = f(x + (-x)) = f(0) = 0$, it also follows that $f(x) = -f(-x)$. In particular, for any natural number $n$, $f(-n) = -f(n) = -cn = c(-n)$.

Moreover, $nf(1/n) = f(1) = c$ which implies that $f(1/n) = c(1/n)$. Consequently, $f(-1/n) = -f(1/n) = c(-1/n)$. Finally, writing any rational number as $m/n$ with a natural number $m$ and integer $n$, $f(m/n) = mf(1/n) = mc/n = c(m/n)$. This proves the statement $f(x) = cx$ for all rational numbers $x$.

\setcounter{subsection}{16}
\subsection{Inequalities on functions of sums and products}

If $f(x) = 0$ for all $x$, then $f$ satisfies $f(x + y) = f(x) + f(y)$ for all $x$ and $y$, and also $f(x \cdot y) = f(x) \cdot f(y)$ for all $x$ and $y$. Now suppose that $f$ satisfies these two properties, but that $f(x)$ is not always 0. Prove that $f(x) = x$ for all $x$, as follows:

\paragraph{Problem (a).} Prove that $f(1) = 1$.

\paragraph{Solution (a).} From the property $f(x \cdot y) = f(x) \cdot f(y)$, \begin{equation*}
  f(1) = f(1 \cdot 1) = f(1) \cdot f(1)
\end{equation*} which implies $f(1) = 0, 1$. However, if $f(1) = 0$, then for any $y$, $f(y) = f(1 \cdot y) = f(1) \cdot f(y) = 0$ which implies that $f(y) = 0$ for all $y$ contrary to the assumption made. Hence, $f(1) = 1$.

\paragraph{Problem (b).} Prove that $f(x) = x$ if $x$ is rational.

\paragraph{Solution (b).} Let $c = f(1)$. The proof that $f(x) = cx$ for all rational $x$ is similar to that in Q16. Since $c = 1$, the statement is proven.

\paragraph{Problem (c) (abridged).} Prove that $f(x) > 0$ if $x > 0$.

\paragraph{Solution (c).} If $x > 0$, then $x = y^2$ for some real $y$, so $f(x) = f(y)^2 = (f(y))^2 \geq 0$ by definition. Since $y \neq 0$ (from (a)), it must follow that $f(y) \neq 0$ and thus $f(x) > 0$.

\paragraph{Problem (d).} Prove that $f(x) > f(y)$ if $x > y$.

\paragraph{Solution (d).} If $x > y$, then $x - y > 0$. By (c), $f(x) - f(y) > 0$, which proves $f(x) > f(y)$.

\paragraph{Problem (e).} Prove that $f(x) = x$ for all $x$.

\paragraph{Solution (e).} Suppose that $f(x) > x$ for some $x$. Choose a rational number $r$ with $x < r < f(x)$. Then, by (b) and (d), \begin{equation*}
  f(x) < f(r) = r < f(x)
\end{equation*} which is a contradiction. Similarly, if $f(x) < x$ for some $x$, by choosing a rational number $r'$ with $f(x) < r' < x$, by (b) and (d), \begin{equation*}
  r' = f(r') < f(x) < r'
\end{equation*} which is a contradiction. Hence, $f(x) = x$ for all $x$.

\setcounter{subsection}{17}
\subsection{Product of functions}

\paragraph{Problem.} Precisely what conditions must $f$, $g$, $h$, and $k$ satisfy in order that $f(x)g(y) = h(x)k(y)$ for all $x$ and $y$?

\paragraph{Solution.} If either $f = 0$ or $g = 0$ holds, and also either $h = 0$ or $k = 0$, then the equation certainly holds. If not, then there exists some $x'$ with $f(x') \neq 0$ and some $y'$ with $g(y') \neq 0$. Then, $0 \neq f(x')g(y') = h(x')k(y')$, so we have $h(x') \neq 0$ and $k(y') \neq 0$. Letting $\alpha = h(x')/f(x')$, $g(y) = \alpha k(y)$ for all $y$. Similarly, from $\alpha = g(y')/k(y')$, $h(x) = \alpha f(x)$ for all $x$. Hence, $h = \alpha f$ and $g = \alpha k$ for some $\alpha \neq 0$.

\setcounter{subsection}{18}
\subsection{More sums and products}

\paragraph{Problem (a) (abridged).} Prove that there do not exist functions $f$ and $g$ with either of the following properties: \begin{align*}
  f(x) + g(y) = xy \text{ for all } x \text{ and } y, \\
  f(x) \cdot g(y) = x + y \text{ for all } x \text{ and } y.
\end{align*}

\paragraph{Solution (a).} Assuming that there exist functions meeting the first condition, $f(x) + g(0) = x \cdot 0 = 0$ for all $x$, so $f(x) = -g(0)$. Likewise, $f(0) + g(y) = 0 \cdot y = 0$ for all $y$, so $g(y) = -f(0) = g(0)$. This would imply that $f(x) + g(y) = -g(0) + g(0) = 0 = xy$ for all $x$ and $y$, which is absurd.

Assuming that there exist functions meeting the second condition, $f(x) \cdot g(0) = x + 0 = x$ for all $x$, so $f(x) = x/g(0)$. Likewise, $f(0) \cdot g(y) = 0 + y = y$ for all $y$, so $g(y) = y/f(0)$. This would imply that $f(x) \cdot g(y) = x/g(0) \cdot y/f(0) = x + y$ for all $x$ and $y$. For $y = 0$, $x = 0$ for all $x$ which is absurd.

\paragraph{Problem (b).} Find functions $f$ and $g$ such that $f(x + y) = g(xy)$ for all $x$ and $y$.

\paragraph{Solution (b).} Let $f$ and $g$ be the same constant function.

\setcounter{subsection}{19}
\subsection{Modulus and squares}

\paragraph{Problem (a).} Find a function $f$, other than a constant function, such that $|f(y) - f(x)| \leq |y - x|$.

\paragraph{Solution (a).} Since $0 \leq |f(y) - f(x)| \leq |y - x|$, the function $f(x) = cx$ for some $0 < c \leq 1$ will satisfy the condition.

\paragraph{Problem (b) (abridged).} Suppose that $f(y) - f(x) \leq (y - x)^2$ for all $x$ and $y$. (Why does this imply that $|f(y) - f(x)| \leq (y - x)^2$?) Prove that $f$ is a constant function.

\paragraph{Solution (b).} Suppose that $f(y) < f(x)$. Naturally, $f(y) - f(x) < 0 \leq (y - x)^2$. Swapping $x$ and $y$, for $f(x) < f(y)$, the statement $0 \leq f(x) - f(y) < (x - y)^2$ must also hold. Hence, $|f(y) - f(x)| = |f(x) - f(y)| \leq (y - x)^2$ for all $x$ and $y$.

Let $m = \frac{x + y}{2}$. Then, $f(y) - f(m) \leq (y - m)^2 = \left(y - \frac{x + y}{2}\right)^2 = \left(\frac{y - x}{2}\right)^2 = \frac{1}{4}(y - x)^2$. Similarly, $f(m) - f(x) \leq (m - x)^2 = \left(\frac{x + y}{2} - x\right)^2 = \left(\frac{y - x}{2}\right)^2 = \frac{1}{4}(y - x)^2$. This suggests that $f(y) - f(x) \leq \frac{1}{2}(y - x)^2$, providing a stricter bound than $(y - x)^2$.

The same process can be repeated indefinitely, with the bound tending towards 0 while remaining positive. Hence, $f(y) - f(x) = 0$ and $f$ is a constant function.

\end{document}

